Convert $\mathcal{P}_2([0,1])$ into an inner product space by writing $\langle p,q \rangle = \int_0^1 p(x)\overline{q(x)} \; dx$ for $p,q \in \mathcal{P}_2([0,1])$. Find a complete orthonormal set in that space.

\nnl \textbf{Solution:} Direct computation via Gram Schmidt.

    \nl Let $\poly{2}{[0,1]}$ have the ordered basis $\set{1,x,x^2}$ denoted by $\set{v_1,v_2,v_3}$. Using the Gram Schmidt process, we will compute $e_1, e_2$ and $e_3$.

    \nnl For $e_1 = \dfrac{v_1}{\norm{v_1}}$, we compute as follows.
    \begin{align*}
        e_1 &= \frac{v_1}{\norm{v_1}}\\ &= \frac{1}{\norm{1}}\\
        &= \over{\inner{1,1}}\\
        &= \over{\int_0^1 1 \cdot 1 \, dx}\\
        &= \over{ x\big|_{x=0}^{x=1}}\\
        &= \over{1-0}\\
        &= 1.
    \end{align*}
    
    \newpage Next, let $\alpha = v_2-\inner{v_2,e_1}e_1$. Then $e_2 = \dfrac{v_2-\inner{v_2,e_1}e_1}{\norm{v_2-\inner{v_2,e_1}e_1}} = \dfrac{\alpha}{\norm{\alpha}}$. Computing $\alpha$,
    \begin{align*}
        \alpha &= v_2-\inner{v_2,e_1}e_1\\
            &= x-\inner{x,1}\cdot 1 \\
            &= x - 1 \int_0^1 1x \,dx\\
            &= x - \brac{\frac{x^2}{2}}_{x=0}^{x=1}\\
            &= x - \over{2}\brac{(1)^2 - (0)^2}\\
            &= x - \over{2}.
    \end{align*}
    And computing the norm,
    \begin{align*}
        \norm{\alpha} &= \norm{x - \over{2}}\\
            &= \sqrt{\inner{x - \over{2}, \; x - \over{2}}}\\
            &= \sqrt{\int_0^1 \pars{x - \over{2}}^2\,dx}\\
            &= \sqrt{\over{3}\brac{\pars{x - \over{2}}^3}_{x=0}^{x=1}}\\
            &= \sqrt{\over{3}\brac{\pars{1 - \over{2}}^3 - \pars{0 - \over{2}}^3}}\\
            &= \sqrt{\over{3}\brac{\over{8} - \pars{- \over{8}}}}\\
            &= \sqrt{\over{12}}\\
            &= \over{2\sqrt{3}}.
    \end{align*}
    And hence,
    \begin{align*}
        e_2 &= \frac{\alpha}{\norm{\alpha}}\\
        &= \frac{x - \over{2}}{\over{2\sqrt{3}}}\\
        &= 2\sqrt{3}\pars{x - \over{2}}.
    \end{align*}
    
    \nl Lastly, let $\beta = v_3 - \inner{v_3,e_1}e_1 - \inner{v_3}{e_2}e_2$. Then $e_3 = \dfrac{\beta}{\norm{\beta}}$. Computing $\beta$,
    \begin{align*}
        \beta &= v_3 - \inner{v_3,e_1}e_1 - \inner{v_3,e_2}e_2\\
        &= x^2 - \inner{x^2, 1} - \inner{x^2, 2\sqrt{3}\pars{x - \over{2}}}\cdot 2\sqrt{3}\pars{x - \over{2}}\\
        &= x^2 - \int_0^1 x^2 \, dx - 2\sqrt{3} \cdot 2\sqrt{3}\pars{x - \over{2}} \int_0^1 \pars{x^3 - \frac{x^2}{2}} \,dx\\
        &= x^2 - \int_0^1 x^2 \, dx - \pars{ 12x-6 } \int_0^1 \pars{x^3 - \frac{x^2}{2}} \,dx\\
        &= x^2 - \brac{\frac{x^3}{3}}_{x=0}^{x=1} - \pars{ 12x-6 } \brac{\frac{x^4}{4} - \frac{x^3}{6}}_{x=0}^{x=1}\\
        &= x^2 - \over{3} - \pars{ 12x-6 } \brac{\over{12}}\\
        &= x^2 - \over{3} - \pars{ x-\over{2} }\\
        &= x^2 - x + \over{6}.
    \end{align*}
    And
    \begin{align*}
        \norm{\beta} &= \sqrt{\inner{\beta, \beta}}\\
        &= \sqrt{\int_0^1 \pars{x^2 - x + \over{6}}^2\,dx}\\
        &= \sqrt{\int_0^1 \pars{x^4 - 2x^3 + \frac 43x^2 -\frac 13x + \over{36}}dx}\\
        &= \sqrt{\brac{\frac{x^5}{5} - \frac{x^4}{2} + \frac{4x^3}{9} - \frac{x^2}{6} + \frac{x}{36} }_{x=0}^{x=1}}\\
        &= \sqrt{\over 5 - \over 2 + \frac{4}{9} - \over{6} + \over{36}}\\
        &= \sqrt{\frac{36-90+80-30+5}{180}}\\
        &= \over{\sqrt{180}}\\
        &= \over{6\sqrt{5}}.
    \end{align*}
    Hence $\displaystyle
        e_3 = \frac{\beta}{\norm{\beta}} = \frac{x^2 - x + \over{6}}{(6\sqrt{5})^{-1}}
        = 6\sqrt{5}\pars{x^2 - x + \over{6}}.$
    Therefore the orthonormal basis of $\poly{2}{[0,1]}$ is
    $$\set{1,\quad 2\sqrt3 \pars{x-\over2}, \quad 6\sqrt{5}\pars{x^2 - x + \over{6}} }.$$
