\begin{align*}
    \inner{u,v} + \inner{v,u} &= \inner{u,v} + \innerc{u,v} \\
    &= \big( \Re\inner{u,v} + \Im \inner{u,v}i \big) + \big( \overline{\Re \inner{u,v}  +  \Im \inner{u,v}i} \big) \\
    &= \big( \Re \inner{u,v} + \Im \inner{u,v}i \big) + \big( \overline{\Re \inner{u,v} } + \overline{ \Im \inner{u,v}i} \big) \\
    &= \big( \Re \inner{u,v} + \Im \inner{u,v}i \big) + \big( \Re \inner{u,v} - \Im \inner{u,v}i \big) \\
    &= 2 \Re \inner{u,v}
\end{align*}

\begin{align*}
    \norm{u+v}^2 &= \norm u^2 + \norm v^2 \\
    &\implies 2 \Re \inner{u,v} = 0 \implies \Re \inner{u,v} = 0
\end{align*}