Suppose $S,T \in \mathcal{L}(V)$ are self-adjoint.  Prove that $ST$ is self-adjoint if and only if $ST = TS$.

\vspace{.1in}

\begin{proof} ($\Longrightarrow$) (If $ST$ is self-adjoint then $ST=TS$.)
\begin{align*}
    ST &= (ST)^* \tag{\text{$ST$ self adjoint hypothesis}}\\
    &= T^* S^* \tag{\text{property e}} \\
    &= TS. \tag{$T = T^*$ \text{ and } $S=S^*$ \text{ hypothesis}}
\end{align*}
Hence if $ST$ is self adjoint then $ST = TS$.
\end{proof}

\vspace{0.3in}
\begin{proof} ($\Longleftarrow$) (If $ST = TS$ then $ST$ is self-adjoint.)
    \begin{align*}
        (ST)^* &= T^*S^* \tag{property e}\\
        &= TS \tag{$T=T^*$ and $S=S^*$ hypothesis}\\
        &= ST. \tag{$ST = TS$ hypothesis}
    \end{align*}
    Hence if $ST = TS$ then $(ST)^*=ST$. In other words, $ST$ is self-adjoint.
    \end{proof}
    